compcomp/val_casted.v
@@ -1,0 +1,297 @@
+(*TODO: These imports should be pared down*)
+Require Import FSets.
+Require FSetAVL.
+Require Import Coqlib.
+Require Import Errors.
+Require Import Ordered.
+Require Import AST.
+Require Import Maps.
+Require Import Integers.
+Require Import Floats.
+Require Import Values.
+Require Import Memory.
+Require Import Globalenvs.
+Require Import Events.
+Require Import Smallstep.
+Require Import Ctypes.
+Require Import Cop.
+Require Import Clight.
+Require Import compcomp.SimplLocals.
+
+Require Import sepcomp.mem_lemmas.
+Require Import sepcomp.core_semantics.
+Require Import sepcomp.core_semantics_lemmas.
+Require Import sepcomp.reach.
+Require Import sepcomp.effect_semantics.
+Require Import StructuredInjections.
+Require Import effect_simulations.
+Require Import sepcomp.effect_properties.
+Require Import effect_simulations_lemmas.
+
+Require Export Axioms.
+
+(** Properties of values obtained by casting to a given type. *)
+
+Inductive val_casted: val -> type -> Prop :=
+  | val_casted_int: forall sz si attr n,
+      cast_int_int sz si n = n ->
+      val_casted (Vint n) (Tint sz si attr)
+  | val_casted_float: forall sz attr n,
+      cast_float_float sz n = n ->
+      val_casted (Vfloat n) (Tfloat sz attr)
+  | val_casted_long: forall si attr n,
+      val_casted (Vlong n) (Tlong si attr)
+  | val_casted_ptr_ptr: forall b ofs ty attr,
+      val_casted (Vptr b ofs) (Tpointer ty attr)
+  | val_casted_int_ptr: forall n ty attr,
+      val_casted (Vint n) (Tpointer ty attr)
+  | val_casted_ptr_int: forall b ofs si attr,
+      val_casted (Vptr b ofs) (Tint I32 si attr)
+  | val_casted_ptr_cptr: forall b ofs id attr,
+      val_casted (Vptr b ofs) (Tcomp_ptr id attr)
+  | val_casted_int_cptr: forall n id attr,
+      val_casted (Vint n) (Tcomp_ptr id attr)
+  | val_casted_struct: forall id fld attr b ofs,
+      val_casted (Vptr b ofs) (Tstruct id fld attr)
+  | val_casted_union: forall id fld attr b ofs,
+      val_casted (Vptr b ofs) (Tunion id fld attr)
+  | val_casted_void: forall v,
+      val_casted v Tvoid.
+
+Definition val_casted_func (v : val) (t : type) : bool :=
+  match v, t with
+    | Vint n, Tint sz si attr => 
+      if Int.eq_dec (cast_int_int sz si n) n then true
+      else false
+    | Vfloat n, Tfloat sz attr => 
+      if Float.eq_dec (cast_float_float sz n) n then true
+      else false
+    | Vlong n, Tlong si attr => true
+    | Vptr b ofs, Tpointer ty attr => true
+    | Vint n, Tpointer ty attr => true
+    | Vptr b ofs, Tint I32 si attr => true
+    | Vptr b ofs, Tcomp_ptr id attr => true
+    | Vint n, Tcomp_ptr id attr => true
+    | Vptr b ofs, Tstruct id flt attr => true
+    | Vptr b ofs, Tunion id flt attr => true
+    | _, Tvoid => true 
+    | _, _ => false
+  end.
+
+Lemma val_casted_funcI v t : 
+  val_casted v t -> 
+  val_casted_func v t=true.
+Proof.
+destruct 1; simpl; auto.
+rewrite H. case_eq (Int.eq_dec n n); auto.
+rewrite H. case_eq (Float.eq_dec n n); auto.
+destruct v; auto.
+Qed.
+
+Lemma val_casted_funcE v t : 
+  val_casted_func v t=true ->
+  val_casted v t.
+Proof.
+destruct v; destruct t; simpl; try solve[inversion 1;econstructor; eauto].
+case_eq (Int.eq_dec (cast_int_int i0 s i) i). intros e _ _.
+constructor; auto. intros n _; inversion 1.
+case_eq (Float.eq_dec (cast_float_float f0 f) f). intros e _ _.
+constructor; auto. intros n _; inversion 1.
+destruct i0; try inversion 1. constructor.
+Qed.
+
+Lemma val_casted_funcP v t : 
+  val_casted_func v t=true <-> val_casted v t.
+Proof.
+split; [apply val_casted_funcE|apply val_casted_funcI].
+Qed.
+
+Remark cast_int_int_idem:
+  forall sz sg i, cast_int_int sz sg (cast_int_int sz sg i) = cast_int_int sz sg i.
+Proof.
+  intros. destruct sz; simpl; auto. 
+  destruct sg; [apply Int.sign_ext_idem|apply Int.zero_ext_idem]; compute; intuition congruence.
+  destruct sg; [apply Int.sign_ext_idem|apply Int.zero_ext_idem]; compute; intuition congruence.
+  destruct (Int.eq i Int.zero); auto.
+Qed.
+
+Remark cast_float_float_idem:
+  forall sz f, cast_float_float sz (cast_float_float sz f) = cast_float_float sz f.
+Proof.
+  intros; destruct sz; simpl.
+  apply Float.singleoffloat_idem; auto.
+  auto.
+Qed.
+
+Lemma cast_val_is_casted:
+  forall v ty ty' v', sem_cast v ty ty' = Some v' -> val_casted v' ty'.
+Proof.
+  unfold sem_cast; intros. destruct ty'; simpl in *.
+(* void *)
+  constructor.
+(* int *)
+  destruct i; destruct ty; simpl in H; try discriminate; destruct v; inv H.
+  constructor. apply (cast_int_int_idem I8 s).
+  constructor. apply (cast_int_int_idem I8 s).
+  destruct (cast_float_int s f0); inv H1.   constructor. apply (cast_int_int_idem I8 s). 
+  constructor. apply (cast_int_int_idem I16 s).
+  constructor. apply (cast_int_int_idem I16 s).
+  destruct (cast_float_int s f0); inv H1.   constructor. apply (cast_int_int_idem I16 s). 
+  constructor. auto.
+  constructor.
+  constructor. auto. 
+  destruct (cast_float_int s f0); inv H1. constructor. auto.
+  constructor. auto.
+  constructor.
+  constructor; auto.
+  constructor.
+  constructor; auto.
+  constructor; auto.
+  constructor; auto.
+  constructor; auto.
+  constructor. simpl. destruct (Int.eq i0 Int.zero); auto.
+  constructor. simpl. destruct (Int64.eq i Int64.zero); auto.
+  constructor. simpl. destruct (Float.cmp Ceq f0 Float.zero); auto.
+  constructor. simpl. destruct (Int.eq i Int.zero); auto.
+  constructor; auto.
+  constructor. simpl. destruct (Int.eq i Int.zero); auto.
+  constructor; auto.
+  constructor. simpl. destruct (Int.eq i Int.zero); auto.
+  constructor; auto.
+  constructor. simpl. destruct (Int.eq i0 Int.zero); auto.
+  constructor; auto.
+(* long *)
+  destruct ty; try discriminate.
+  destruct v; inv H. constructor.
+  destruct v; inv H. constructor.
+  destruct v; try discriminate. destruct (cast_float_long s f0); inv H. constructor.
+  destruct v; inv H. constructor.
+  destruct v; inv H. constructor.
+  destruct v; inv H. constructor.
+  destruct v; inv H. constructor.
+(* float *)
+  destruct ty; simpl in H; try discriminate; destruct v; inv H.
+  constructor. unfold cast_float_float, cast_int_float.
+  destruct f; destruct s; auto.
+  rewrite Float.singleofint_floatofint. apply Float.singleoffloat_idem.
+  rewrite Float.singleofintu_floatofintu. apply Float.singleoffloat_idem.
+  constructor. unfold cast_float_float, cast_long_float.
+  destruct f; destruct s; auto. apply Float.singleoflong_idem. apply Float.singleoflongu_idem.
+  constructor. apply cast_float_float_idem.
+(* pointer *)
+  destruct ty; simpl in H; try discriminate; destruct v; inv H; try constructor.
+(* impossible cases *)
+  discriminate.
+  discriminate.
+(* structs *)
+  destruct ty; try discriminate; destruct v; try discriminate.
+  destruct (ident_eq i0 i && fieldlist_eq f0 f); inv H; constructor.
+(* unions *)
+  destruct ty; try discriminate; destruct v; try discriminate.
+  destruct (ident_eq i0 i && fieldlist_eq f0 f); inv H; constructor.
+(* comp_ptr *)
+  destruct ty; simpl in H; try discriminate; destruct v; inv H; constructor.
+Qed.
+
+Lemma val_casted_load_result:
+  forall v ty chunk,
+  val_casted v ty -> access_mode ty = By_value chunk ->
+  Val.load_result chunk v = v.
+Proof.
+  intros. inversion H; clear H; subst v ty; simpl in H0.
+  destruct sz.
+  destruct si; inversion H0; clear H0; subst chunk; simpl in *; congruence.
+  destruct si; inversion H0; clear H0; subst chunk; simpl in *; congruence.
+  clear H1. inv H0. auto.
+  inversion H0; clear H0; subst chunk. simpl in *. 
+  destruct (Int.eq n Int.zero); subst n; reflexivity.
+  destruct sz; inversion H0; clear H0; subst chunk; simpl in *; congruence.
+  inv H0; auto.
+  inv H0; auto.
+  inv H0; auto.
+  inv H0; auto.
+  discriminate.
+  discriminate.
+  discriminate.
+  discriminate.
+  discriminate.
+Qed.
+
+Lemma cast_val_casted:
+  forall v ty, val_casted v ty -> sem_cast v ty ty = Some v.
+Proof.
+  intros. inversion H; clear H; subst v ty; unfold sem_cast; simpl; auto.
+  destruct sz; congruence.
+  congruence.
+  unfold proj_sumbool; repeat rewrite dec_eq_true; auto.
+  unfold proj_sumbool; repeat rewrite dec_eq_true; auto.
+Qed.
+
+Lemma val_casted_inject:
+  forall f v v' ty,
+  val_inject f v v' -> val_casted v ty -> val_casted v' ty.
+Proof.
+  intros. inv H; auto.
+  inv H0; constructor.
+  inv H0; constructor.
+Qed.
+
+Inductive val_casted_list: list val -> typelist -> Prop :=
+  | vcl_nil:
+      val_casted_list nil Tnil
+  | vcl_cons: forall v1 vl ty1 tyl,
+      val_casted v1 ty1 -> val_casted_list vl tyl ->
+      val_casted_list (v1 :: vl) (Tcons  ty1 tyl).
+
+Lemma val_casted_list_params:
+  forall params vl,
+  val_casted_list vl (type_of_params params) ->
+  list_forall2 val_casted vl (map snd params).
+Proof.
+  induction params; simpl; intros. 
+  inv H. constructor.
+  destruct a as [id ty]. inv H. constructor; auto. 
+Qed.
+
+Fixpoint val_casted_list_func (vs : list val) (ts : typelist) : bool :=
+  match vs, ts with
+    | nil, Tnil => true
+    | v1 :: vl, Tcons ty1 tyl => 
+      val_casted_func v1 ty1 && val_casted_list_func vl tyl
+    | _, _ => false
+  end.
+
+Lemma val_casted_list_funcP vs ts : 
+  val_casted_list_func vs ts=true <-> val_casted_list vs ts.
+Proof.
+revert ts; induction vs. destruct ts; simpl; auto.
+split; auto. intros _. constructor.
+split; auto. inversion 1. inversion 1.
+split; auto. destruct ts; simpl; auto.
+inversion 1. rewrite andb_true_iff. intros [H1 H2]. constructor.
+apply val_casted_funcE in H1; auto. rewrite <-IHvs; auto.
+inversion 1; subst. simpl. rewrite andb_true_iff; split.
+apply val_casted_funcI; auto. rewrite IHvs; auto.
+Qed.
+
+Lemma val_casted_inj (j : meminj) v1 v2 tv : 
+  val_inject j v1 v2 -> 
+  val_casted v1 tv -> 
+  val_casted v2 tv.
+Proof.
+inversion 1; subst; auto.
+inversion 1; subst; auto; try solve[constructor; auto].
+inversion 1; constructor.
+Qed.
+
+Lemma val_casted_list_inj (j : meminj) vs1 vs2 ts :
+  val_list_inject j vs1 vs2 ->
+  val_casted_list vs1 ts ->
+  val_casted_list vs2 ts.
+Proof.
+intros H1; revert vs1 vs2 H1; induction ts; simpl; intros vs1 vs2 H1 H2.
+revert H2 H1; inversion 1; subst. inversion 1; subst. constructor.
+revert H2 H1; inversion 1; subst. inversion 1; subst. constructor.
+eapply val_casted_inj; eauto.
+eapply IHts; eauto.
+Qed.
